update composition rules

compcertox/Composition.v
@@ -6,102 +6,56 @@ From compcert.lib Require Import
      Coqlib.
 From compcert.common Require Import
      LanguageInterface
-     Events
-     Globalenvs
-     Smallstep
-     Linking
+     Events Globalenvs
+     Smallstep Linking
      Memory Values
      CallconvAlgebra
      CategoricalComp
      FlatComp.
 From compcert.cfrontend Require Import
-     Clight
-     Ctypes.
+     Clight Ctypes.
 From compcertox Require Import
-     Lifting
-     AbstractStateRel
-     CModule
-     TensorComp.
+     Lifting AbRel
+     CModule TensorComp.
 
 (* FIXME: why the precedence can't be looser than 9? *)
-Notation "[ R ]" := (singleton_rel R) (at level 9): krel_scope.
+(* Notation "[ R ]" := (singleton_rel R) (at level 9): krel_scope. *)
 
-Section PROG_LAYER_DEF.
-  (* L1 is the high level spec with K1 as the abstract data whereas the program
-     running on top of L2 is the low level spec *)
-  Context {K1 K2: Type} (L1: layer K1) (L2: layer K2) (p: Clight.program).
+Generalizable All Variables.
 
-  Definition prog_layer_comp sk := comp_semantics' (Clight.semantics2 p @ K2) L2 sk.
+(** ** Definitions for CAL in CompCertOX *)
 
-  (* The version of certified abstraction layers for vertical composition *)
-  Definition prog_ksim (R: crel K1 K2) :=
-    linkorder (skel L2) (skel L1) /\ linkorder (AST.erase_program p) (skel L1) /\
-    forward_simulation 1 R L1 (prog_layer_comp (skel L1)).
+Section LAYER_DEF.
+  (* Ls is the high level spec with Ks as the abstract data whereas the program
+     running on top of Lf is the low level spec *)
+  Context {Ks Kf} (Ls: layer Ks) (Lf: layer Kf).
 
-  (* The version that is horizontally compositional *)
-  Definition prog_ksim_mcc (R: krel K1 K2) :=
-    linkorder (skel L2) (skel L1) /\ linkorder (AST.erase_program p) (skel L1) /\
-    forward_simulation 1 (krel_mcc R) L1 (prog_layer_comp (skel L1)).
+  Section PROG.
+    Context (p: Clight.program).
+    Definition prog_layer_comp sk := comp_semantics' (Clight.semantics2 p @ Kf) Lf sk.
+    Definition prog_sim (R: abrel Ks Kf) :=
+      linkorder (skel Lf) (skel Ls) /\ linkorder (AST.erase_program p) (skel Ls) /\
+        forward_simulation 1 R Ls (prog_layer_comp (skel Ls)).
+  End PROG.
 
-  Lemma prog_ksim_ref (R: krel K1 K2): prog_ksim_mcc R -> prog_ksim [R].
-  Proof.
-    unfold prog_ksim, prog_ksim_mcc. intuition.
-    apply layer_fsim_refine. auto.
-  Qed.
-End PROG_LAYER_DEF.
+  Section CMOD.
+    Context (M: cmodule).
+    Definition layer_comp sk := comp_semantics' (semantics M sk @ Kf) Lf sk.
+    Definition sim (R: abrel Ks Kf) :=
+      linkorder (skel Lf) (skel Ls) /\ skel_module_compatible M (skel Ls) /\
+        forward_simulation 1 R Ls (layer_comp (skel Ls)).
 
-Section MOD_LAYER_DEF.
+  End CMOD.
 
-  Context {K1 K2: Type} (L1: layer K1) (L2: layer K2) (M: cmodule).
-
-  Definition layer_comp sk := comp_semantics' (semantics M sk @ K2) L2 sk.
-
-  Definition ksim (R: crel K1 K2) :=
-    linkorder (skel L2) (skel L1) /\ skel_module_compatible M (skel L1) /\
-    forward_simulation 1 R L1 (layer_comp (skel L1)).
-
-  Definition ksim_mcc (R: krel K1 K2) :=
-    linkorder (skel L2) (skel L1) /\ skel_module_compatible M (skel L1) /\
-    forward_simulation 1 R L1 (layer_comp (skel L1)).
-
-  Definition ksim_ref (R: krel K1 K2): ksim_mcc R -> ksim [R].
-  Proof.
-    unfold ksim, ksim_mcc. intuition.
-    apply layer_fsim_refine. auto.
-  Qed.
-
-End MOD_LAYER_DEF.
-
+End LAYER_DEF.
 
 (* "M:Y" part should have higher priority than the type annotation "a:T" which
    is at level 100 *)
-Notation " X ⊢ [ R ] M : Y " := (ksim_mcc Y X M R) (at level 85, M at level 99).
-Notation " X ⊢ { R } M : Y " := (ksim Y X M R) (at level 85, M at level 99).
+Notation " X ⊢ [ R ] M : Y " := (sim Y X M R) (at level 85, M at level 99).
 
-Instance ksim_mcc_proper {K1 K2: Type}:
-  Proper ((forward_simulation 1 1) --> (forward_simulation 1 1) ==> eq  ==> eq ==> impl) (@ksim_mcc K1 K2).
-Proof.
-  intros L2 L2' HL2 L1 L1' HL1 M N Hmn R S Hrs H.
-  unfold impl, flip in *. subst. destruct H as (?&?&?). split; [| split].
-  - destruct HL1. destruct X.
-    destruct HL2. destruct X. congruence.
-  - destruct HL2. destruct X. congruence.
-  - eapply open_fsim_ccref. apply cc_compose_id_left.
-    unfold flip. apply cc_compose_id_left.
-    eapply compose_forward_simulations. eauto.
-
-    eapply open_fsim_ccref. apply cc_compose_id_left.
-    unfold flip. apply cc_compose_id_right.
-    eapply compose_forward_simulations. eauto.
-
-    destruct HL2. destruct X. rewrite fsim_skel.
-    unfold layer_comp.
-    eapply categorical_compose_simulation';
-      [ reflexivity | assumption | apply linkorder_refl | assumption ].
-Qed.
-
-Instance ksim_monotonic {K1 K2: Type}:
-  Proper ((forward_simulation 1 1) --> (forward_simulation 1 1) ==> eq  ==> eq ==> impl) (@ksim K1 K2).
+Instance sim_monotonic {Ks Kf: Type}:
+  Proper ((forward_simulation 1 1) --> (forward_simulation 1 1) ==> eq  ==> eq ==> impl)
+         (@sim Ks Kf).
 Proof.
   intros L2 L2' HL2 L1 L1' HL1 M N Hmn R S Hrs H.
   unfold impl, flip in *. subst. destruct H as (?&?&?). split; [| split].
@@ -127,6 +81,8 @@ Goal forall K1 K2 (L1: layer K1) (L2: layer K2) R M L2',
 Proof.
   intros * H HL2. now rewrite HL2.
 Qed.
+
+(** *** Promoting a Clight program into a singleton CModule *)
 
 Section HCOMP_SINGLETON.
 
@@ -162,9 +118,9 @@ Section HCOMP_SINGLETON.
 
 End HCOMP_SINGLETON.
 
-Lemma singleton_ksim {K1 K2} L1 L2 p (R: crel K1 K2): prog_ksim L1 L2 p R -> ksim L1 L2 (p :: nil) R.
+Lemma singleton_sim `(R: abrel Ks Kf) Ls Lf p : prog_sim Ls Lf p R -> sim Ls Lf (p :: nil) R.
 Proof.
-  unfold prog_ksim, ksim. intuition.
+  unfold prog_sim, sim. intuition.
   - unfold skel_module_compatible. rewrite Forall_forall.
     intros x Hx. cbn in Hx. destruct Hx; intuition. subst. auto.
   - unfold layer_comp. unfold semantics. unfold ref. cbn.
@@ -174,12 +130,15 @@ Proof.
     eapply compose_forward_simulations. eauto.
 
     unfold prog_layer_comp.
-    etransitivity. apply lift_comp_component3 with (sk1 := (skel L1)).
+    etransitivity. apply lift_comp_component3 with (sk1 := (skel Ls)).
     eapply categorical_compose_simulation'; [ | reflexivity | apply linkorder_refl | auto].
-    replace (skel_extend (semantics2 p @ K2) (skel L1))
-      with (skel_extend (semantics2 p) (skel L1) @ K2) by reflexivity.
-    apply lifting_simulation. apply hcomp_singleton_fsim. typeclasses eauto.
+    replace (skel_extend (semantics2 p @ Kf) (skel Ls))
+      with (skel_extend (semantics2 p) (skel Ls) @ Kf) by reflexivity.
+    apply lifting_simulation. apply hcomp_singleton_fsim.
+    typeclasses eauto.
 Qed.
+
+(** *** Auxiliaries *)
 
 Lemma compatible_app sk M N:
   skel_module_compatible M sk -> skel_module_compatible N sk ->
@@ -213,31 +172,35 @@ Section SKEL_EXT.
   Qed.
 End SKEL_EXT.
 
+(** ** Composition Rules  *)
+
+(** *** Vertical Composition *)
+
 Section VCOMP.
 
-  Context {K1 K2 K3 L1 L2 L3} {M N: cmodule} {R: crel K1 K2} {S: crel K2 K3}
-          (HL1: ksim L1 L2 M R) (HL2: ksim L2 L3 N S).
-  (* FIXME: the linkable hypothesis should be simplified *)
-  Context `{!CategoricalLinkable (semantics M (skel L1)) (semantics N (skel L1))}.
+  Context `{R: abrel Ks Kn} `{S: abrel Kn Kf} {M N: cmodule}
+          `(HL1: sim Ls Ln M R) `(HL2: sim Ln Lf N S).
+  Hypothesis HR: disjoint_abrel R S.
+  Context `{!CategoricalLinkable (semantics M (skel Ls)) (semantics N (skel Ls))}.
 
-  Theorem layer_vcomp: ksim L1 L3 (M ++ N) (R ∘ S).
+  Theorem layer_vcomp: sim Ls Lf (M ++ N) (R @ S).
   Proof.
-    unfold ksim in *.
+    unfold sim in *.
     destruct HL1 as [Hsk1 [Hmod1 H1]]. clear HL1.
     destruct HL2 as [Hsk2 [Hmod2 H2]]. clear HL2.
     split. eapply linkorder_trans; eauto.
     split. apply compatible_app; eauto.
     eapply compatible_trans; eauto.
 
-    edestruct (cmodule_krel S M (skel L1)). auto.
+    edestruct (cmodule_abrel S M (skel Ls)). auto.
     exploit @categorical_compose_simulation'.
     constructor. exact X. apply H2.
-    instantiate (1 := (skel L1)). apply linkorder_refl. auto.
+    instantiate (1 := (skel Ls)). apply linkorder_refl. auto.
     clear X. intros X.
 
     eapply open_fsim_ccref. apply cc_compose_id_left.
-    unfold flip. reflexivity.
-    cbn. eapply compose_forward_simulations.
+    unfold flip. apply krel_comp_ref; eauto.
+    eapply compose_forward_simulations.
     apply H1. unfold layer_comp.
 
     eapply open_fsim_ccref. apply cc_compose_id_left.
@@ -265,9 +228,11 @@ Section VCOMP.
 
 End VCOMP.
 
+(** *** Horizontal Composition *)
+
 Lemma layer_comp_extend_skel {K} M L sk sk':
   linkorder sk' sk -> linkorder (skel L) sk ->
-  skel_extend (layer_comp L M sk') sk ≤ layer_comp (K2 := K) L M sk.
+  skel_extend (layer_comp L M sk') sk ≤ layer_comp (Kf := K) L M sk.
 Proof.
   unfold layer_comp.
   replace (skel_extend (comp_semantics' (semantics M sk' @ K) L sk') sk)
@@ -286,19 +251,18 @@ Qed.
 
 Section HCOMP.
 
-  Generalizable All Variables.
-  Context `{R: crel K1 K2} {M N: cmodule} `(HL1: ksim L1 L3 M R) `(HL2: ksim L2 L3 N R).
+  Context `{R: abrel Ks Kf} {M N: cmodule} `(HL1: sim Ls1 Lf M R) `(HL2: sim Ls2 Lf N R).
   Variable (sk: AST.program unit unit).
-  Hypothesis (Hk1: linkorder (skel L1) sk)
-             (Hk2: linkorder (skel L2) sk).
+  Hypothesis (Hk1: linkorder (skel Ls1) sk)
+             (Hk2: linkorder (skel Ls2) sk).
   Let Mi := (fun i : bool => if i then semantics M sk else semantics N sk).
   Context `{!FlatLinkable Mi}.
 
-  Let L i := match i with true => L1 | false => L2 end.
+  Let L i := match i with true => Ls1 | false => Ls2 end.
 
-  Theorem layer_hcomp: ksim (flat_comp_semantics' L sk) L3 (M ++ N) R.
+  Theorem layer_hcomp: sim (flat_comp_semantics' L sk) Lf (M ++ N) R.
   Proof.
-    unfold ksim in *.
+    unfold sim in *.
     destruct HL1 as [Hsk1 [Hmod1 H1]]. clear HL1.
     destruct HL2 as [Hsk2 [Hmod2 H2]]. clear HL2.
     split. eapply linkorder_trans; eauto.
@@ -308,8 +272,8 @@ Section HCOMP.
     unfold flip. apply cc_compose_id_right.
     eapply compose_forward_simulations.
 
-    set (Ls := fun i => match i with true => layer_comp L3 M (skel L1)
-                             | false => layer_comp L3 N (skel L2) end).
+    set (Ls := fun i => match i with true => layer_comp Lf M (skel Ls1)
+                             | false => layer_comp Lf N (skel Ls2) end).
     apply (flat_composition_simulation' _ _ _ Ls); try (intros [|]; auto). cbn.
 
     (* To use the distributivity, we first unify the code skeleton of the
@@ -317,7 +281,7 @@ Section HCOMP.
     etransitivity. apply lift_flat_comp_component. cbn.
     rewrite if_rewrite with (f := fun x => skel_extend x sk).
 
-    set (Ls := fun i => match i with true => layer_comp L3 M sk | false => layer_comp L3 N sk end).
+    set (Ls := fun i => match i with true => layer_comp Lf M sk | false => layer_comp Lf N sk end).
     etransitivity. instantiate (1 := flat_comp_semantics' Ls sk).
     {
       apply flat_composition_simulation'.
@@ -327,7 +291,7 @@ Section HCOMP.
     }
 
     subst Ls. unfold layer_comp.
-    rewrite <- if_rewrite with (f := fun x => comp_semantics' x L3 sk).
+    rewrite <- if_rewrite with (f := fun x => comp_semantics' x Lf sk).
     etransitivity.  apply distributivity2. constructor. exact true.
     eapply categorical_compose_simulation';
       [ | apply identity_forward_simulation
@@ -342,23 +306,23 @@ Section HCOMP.
 
 End HCOMP.
 
+(** *** Tensor Product *)
+
 Section TCOMP.
 
-  Context {K1 K2 K3 K4: Type} (R: krel K1 K2) (S: krel K3 K4).
-  Context (L1: layer K1) (L2: layer K2) (L3: layer K3) (L4: layer K4).
-  Context (M N: cmodule).
-  Hypothesis (HL1: L2 ⊢ [R] M : L1) (HL2: L4 ⊢ [S] N : L3).
+  Context `(R1: abrel Ks1 Kf1) `(R2: abrel Ks2 Kf2) (M N: cmodule).
+  Context `(HL1: Lf1 ⊢ [R1] M : Ls1) `(HL2: Lf2 ⊢ [R2] N : Ls2).
   Variable (sk_lo sk_hi: AST.program unit unit).
-  Hypothesis (Hsk1: linkorder (skel L2) sk_lo) (Hsk2: linkorder (skel L4) sk_lo)
-             (Hsk3: linkorder (skel L1) sk_hi) (Hsk4: linkorder (skel L3) sk_hi)
+  Hypothesis (Hsk1: linkorder (skel Lf2) sk_lo) (Hsk2: linkorder (skel Lf2) sk_lo)
+             (Hsk3: linkorder (skel Ls1) sk_hi) (Hsk4: linkorder (skel Ls2) sk_hi)
              (Hsk: linkorder sk_lo sk_hi).
   Let Mi := (fun i : bool => if i then semantics M sk_hi else semantics N sk_hi).
   Context `{!FlatLinkable Mi}.
-  Hypothesis Hdisjoint: forall i, vars S i -> vars R i -> False.
+  Hypothesis HR: disjoint_abrel R1 R2.
 
-  Lemma layer_tcomp: ksim_mcc (tensor_comp_semantics' L1 L3 sk_hi)
-                              (tensor_comp_semantics' L2 L4 sk_lo)
-                              (M ++ N) (R * S).
+  Lemma layer_tcomp: sim (tensor_comp_semantics' Ls1 Ls2 sk_hi)
+                         (tensor_comp_semantics' Lf1 Lf2 sk_lo)
+                         (M ++ N) (R1 * R2).
   Proof.
     destruct HL1 as [HLsk1 [Hmod1 H1]]. clear HL1.
     destruct HL2 as [HLsk2 [Hmod2 H2]]. clear HL2.
@@ -377,7 +341,7 @@ Section TCOMP.
     {
       apply flat_composition_simulation'. instantiate (1 := fun i => match i with true => _ | false => _ end).
       intros [|].
-      - instantiate (1 := comp_semantics' (semantics M (skel L1) @ (K2 * K4)) (lift_layer_k L2) (skel L1)).
+      - instantiate (1 := comp_semantics' (semantics M (skel Ls1) @ (Kf1 * Kf2)) (lift_layer_k Lf1) (skel Ls1)).
         etransitivity.
         + apply mapB_monotonicity. etransitivity.
           * apply mapA_monotonicity. apply lift_categorical_comp1.
@@ -389,7 +353,7 @@ Section TCOMP.
             -- reflexivity.
             -- apply linkorder_refl.
             -- auto.
-      - instantiate (1 := comp_semantics' (semantics N (skel L3) @ (K2 * K4)) (layer_comm (lift_layer_k L4)) (skel L3)).
+      - instantiate (1 := comp_semantics' (semantics N (skel Ls2) @ (Kf1 * Kf2)) (layer_comm (lift_layer_k Lf2)) (skel Ls2)).
         etransitivity.
         + apply mapB_monotonicity. etransitivity.
           * apply mapB_monotonicity. etransitivity.
@@ -408,9 +372,9 @@ Section TCOMP.
       - intros [|]; auto.
     }
 
-    set (LX:= fun i:bool => if i then semantics M (skel L1) @ (K2 * K4) else semantics N (skel L3) @ (K2 * K4)).
-    set (LY:= fun i:bool => if i then lift_layer_k L2 else layer_comm (lift_layer_k L4)).
-    set (Lsk:= fun i:bool => if i then skel L1 else skel L3).
+    set (LX:= fun i:bool => if i then semantics M (skel Ls1) @ (Kf1 * Kf2) else semantics N (skel Ls2) @ (Kf1 * Kf2)).
+    set (LY:= fun i:bool => if i then lift_layer_k Lf1 else layer_comm (lift_layer_k Lf2)).
+    set (Lsk:= fun i:bool => if i then skel Ls1 else skel Ls2).
     replace (flat_comp_semantics' _ sk_hi) with (flat_comp_semantics' (fun i:bool => comp_semantics' (LX i) (LY i) (Lsk i)) sk_hi).
     2: {
       subst LX  LY Lsk. cbn. f_equal. apply Axioms.functional_extensionality.
@@ -420,7 +384,7 @@ Section TCOMP.
     etransitivity. apply categorical_flat_interchangeable.
     etransitivity; [ | eapply lift_comp_component2 with (sk2 := sk_hi)].
     eapply categorical_compose_simulation'; [ | reflexivity | apply linkorder_refl | apply linkorder_refl ].
-    subst LX. rewrite <- if_rewrite with (f := fun x => x @ (K2 * K4)).
+    subst LX. rewrite <- if_rewrite with (f := fun x => x @ (Kf1 * Kf2)).
     etransitivity. apply lift_flat_comp2. apply lifting_simulation.
     etransitivity. 2: { apply cmodule_flat_comp_simulation. eauto. }
     etransitivity. apply lift_flat_comp_component. cbn.
@@ -429,7 +393,11 @@ Section TCOMP.
 
 End TCOMP.
 
-(* A composition of krel for absfun and bottom layers *)
+(** ** Obsolete Code *)
+
+(** *** A specicial case for compositing absfun and getter-setter layers *)
+
+(*
 Import AbstractStateRel.
 
 Class BotRel {K1 K2: Type} (R: krel K1 K2) :=
@@ -615,7 +583,10 @@ Section ABSFUN.
   Qed.
 
 End ABSFUN.
+ *)
 
+(** *** A special case for pure refinement *)
+(*
 Section PUREREF.
 
   Context {K1 K2 K3 L1 L2 L3} (M: cmodule)
@@ -639,7 +610,9 @@ End PUREREF.
 Instance prod_bot_rel {K1 K2 K3 K4} (R1: krel K1 K2) (R2: krel K3 K4)
          `(!BotRel R1) `(!BotRel R2): BotRel (R1 * R2).
 Proof. intros [k1 k3] [k2 k4]. split; eauto. Qed.
+ *)
 
+(** ** An instance of empty layer *)
 Section NULL.
   Context {K: Type}.
 
